Groups: proved size equality

groups.v
@@ -1409,6 +1409,39 @@ Section finite_groups.
       (forall a, exists b, In a (f b)) ->
       fn_partition A l f.
 
+  Inductive fn_partition_inverse (A: Type) (l: list A) (f: A -> list A) (f_inv: A -> A) :=
+  | fn_partition_inverse_intro:
+      (forall e, In e (f (f_inv e))) ->
+      (*(forall d, In (f_inv d) l) ->*)
+      fn_partition_inverse A l f f_inv.
+
+  Lemma fn_partition_inverse_cons (A: Type) (l: list A) (f: A -> list A) (f_inv: A -> A):
+    forall a, fn_partition_inverse A (a :: l) f f_inv -> fn_partition_inverse A l f f_inv.
+    intros; auto.
+    apply fn_partition_inverse_intro.
+    destruct H0; auto.
+  Qed.
+
+
+  (* func_pair objects func_pair f a *)
+  (* fst (func_pair f a) = a *)
+  (* snd (func_pair f a) = (f a) *)
+
+  Inductive fpair (A: Type) (f: A -> A) :=
+  | fpair_intro: A -> fpair A f.
+
+  Definition fpair_fst (A: Type) (f: A -> A) (p: fpair A f) :=
+    match p with
+    | fpair_intro _ _ a => (f a)
+    end.
+  Definition fpair_snd (A: Type) (f: A -> A) (p: fpair A f) :=
+    match p with
+    | fpair_intro _ _ a => a
+    end.
+
+  Arguments fpair_intro {A} _ _.
+  Hint Constructors fpair.
+
   Theorem unique_cosets_is_partition  (G: finite_group) (H: subgroup G) group_eq_dec:
     fn_partition G (unique_cosets G H group_eq_dec) (finite_coset G H).
   Proof.
@@ -1416,13 +1449,26 @@ Section finite_groups.
     - unfold unique_cosets.
   Admitted.
 
+  Definition expand_partition (A: Type) (l: list A) (f: A -> list A) (f_inv: A -> A) :=
+    flat_map (fun (x : A) => map (fun y => fpair_intro f_inv y) (f x)) l.
+
+(*
   Definition expand_partition (A: Type) (l: list A) (f: A -> list A) :=
     flat_map (fun (x : A) => map (fun y => pair x y) (f x)) l.
+ *)
+    Check (let G := klein_group_finite in
+          let H := klein_subgroup_X in
+          let group_eq_dec := klein_group_eq_decidable in
+          let f := finite_coset G H in
+          let f_inv := canonical_right_coset G H in
+          expand_partition G (unique_cosets G H group_eq_dec) f f_inv).
 
   Compute (let G := klein_group_finite in
           let H := klein_subgroup_X in
           let group_eq_dec := klein_group_eq_decidable in
-          expand_partition G (unique_cosets G H group_eq_dec) (finite_coset G H)).
+          let f := finite_coset G H in
+          let f_inv := canonical_right_coset G H in
+          (map (fpair_fst G f_inv) (expand_partition G (unique_cosets G H group_eq_dec) f f_inv))).
 
   Lemma in_not_append: forall (A: Type) (l1 l2: list A) a,
       ~ In a l1 -> ~ In a l2 -> ~ In a (l1 ++ l2).
@@ -1447,26 +1493,33 @@ Section finite_groups.
      (i.e. it is a partition). *)
 
   Lemma in_concat_map: forall (A B: Type) (f: A -> list B) b (l: list A),
-      In b (concat (map f l)) -> exists a, In b (f a) /\ In a l.
+      In b (concat (map f l)) <-> exists a, In b (f a) /\ In a l.
   Proof.
     intros A B f b.
-    induction l; simpl.
+    induction l; simpl; split.
     - intros H; contradict H; auto.
+    - intros H; destruct H; tauto.
     - intros In_b.
       apply in_app_or in In_b.
       destruct In_b as [b_in_f_a | b_in_rest];
         [exists a | apply IHl in b_in_rest; destruct b_in_rest as [d def_d]; exists d];
         tauto.
+    - intros [a0 [H1 H2]].
+      apply in_or_app.
+      destruct H2 as [a_first | a_rest];
+        [left; rewrite a_first | right; apply IHl; exists a0]; auto.
   Qed.
 
-  Theorem expand_partition_NoDup (A: Type) (l: list A) (f: A -> list A) :
-    fn_partition A l f -> NoDup (expand_partition A l f).
+  Theorem expand_partition_NoDup (A: Type) (l: list A) (f: A -> list A) (f_inv: A -> A):
+    fn_partition A l f ->
+    fn_partition_inverse A l f f_inv ->
+    NoDup (expand_partition A l f f_inv).
   Proof.
-    intros [l_NoDup _ _ NoRepeat _].
+    intros [l_NoDup NoOverlap _ NoRepeat _].
+    intros PartitionInverse.
     unfold expand_partition.
     rewrite flat_map_concat_map.
-    remember (fun x : A => map (fun y : A => (x, y)) (f x)) as inj.
-
+    remember (fun x : A => map (fun y : A => fpair_intro f_inv y) (f x)) as inj.
     induction l; simpl.
     apply NoDup_nil.
     apply NoDup_append.
@@ -1474,6 +1527,7 @@ Section finite_groups.
       [intros x y H; inversion H | apply NoRepeat]; auto.
     apply IHl.
     apply NoDup_cons_iff in l_NoDup; destruct l_NoDup; auto.
+    apply fn_partition_inverse_cons in PartitionInverse; auto.
     intros q.
     destruct q as [x y].
     intros xy_a.
@@ -1484,51 +1538,121 @@ Section finite_groups.
     destruct d_in_rest as [xy_d d_in_rest].
     rewrite Heqinj, in_map_iff in xy_a.
     rewrite Heqinj, in_map_iff in xy_d.
-    destruct xy_a as [r [a_def _]].
-    destruct xy_d as [s [d_def _]].
+    destruct xy_a as [r [a_def a_in]].
+    destruct xy_d as [s [d_def d_in]].
     inversion a_def.
     inversion d_def.
-    rewrite <- H3 in H1.
-    rewrite H1 in l_NoDup.
+    rewrite H1 in a_in.
+    rewrite H2 in d_in.
+    rewrite (NoOverlap _ _ _ a_in d_in) in l_NoDup.
     rewrite NoDup_cons_iff in l_NoDup.
     destruct l_NoDup; auto.
   Qed.
 
-  Theorem expand_partition_listing (
+  Check expand_partition.
 
+  Lemma in_not_exists_in_empty_list (A: Type): ~ (exists a : A, In a []).
+  Proof.
+    intros NonEmpty.
+    destruct NonEmpty as [q NonEmpty]; apply in_nil in NonEmpty; auto.
+  Qed.
+
+  Theorem expand_partition_in  (A: Type) (l: list A) f f_inv:
+    fn_partition A l f ->
+    fn_partition_inverse A l f f_inv ->
+    (forall d, In (f_inv d) l) ->
+    forall c, In c (expand_partition A l f f_inv) <->
+              (exists d, fpair_fst _ _ c = (f_inv d) /\ fpair_snd _ _ c = d).
+  Proof.
+    intros [l_NoDup NoOverlap _ NoRepeat EveryElementInPartition].
+    intros PartitionInverse InverseMapsToList.
+    intros q.
+    unfold expand_partition.
+    rewrite flat_map_concat_map, in_concat_map.
+    split.
+    - intros [a a_in_concatmap].
+      rewrite in_map_iff in a_in_concatmap.
+      destruct a_in_concatmap as [[e [def_e e_in_fa]] a_in_l].
+      rewrite <- def_e.
+      simpl.
+      exists e.
+      tauto.
+    - intros [d d_has_form].
+      exists (f_inv d).
+      rewrite in_map_iff.
+      destruct q.
+      destruct d_has_form as [Q1 Q2].
+      rewrite <- Q1.
+      simpl.
+      split.
+      exists a.
+      split; [reflexivity | apply PartitionInverse].
+      (* must show f_inv a maps into l which is an issue with some of our induction steps *)
+      apply InverseMapsToList.
+  Qed.
+
+  (*
+In c (expand_partition A l f f_inv) <->
+              (exists d, fpair_fst _ _ c = (f_inv d) /\ fpair_snd _ _ c = d) *)
+
+  Theorem expand_partition_listing (A: Type) (l: list A) f f_inv (seq_A: list A):
+    Listing seq_A ->
+    fn_partition A l f ->
+    fn_partition_inverse A l f f_inv ->
+    (forall d, In (f_inv d) l) ->
+    forall c, In c (expand_partition A l f f_inv) <-> In (fpair_snd _ _ c) seq_A.
+  Proof.
+    intros seq_listing Partition PartitionInverse InverseMapsToList.
+    intros d.
+    rewrite (expand_partition_in _ _ f f_inv); auto.
+    split; [intros; apply seq_listing | ].
+    intros in_seq.
+    destruct d.
+    simpl; exists a; tauto.
+  Qed.
+
+  (* at some point must use l nonempty *)
+  (*
+     expand_partition A l f is A * A
+     |
+     | maps to
+     |
+     V
+     seq A
+
+     Issue is that A * A is not the domain of the function
+     (there are many A * A that appear in the type that won't be in the expand_partition list).
+     We should define a different type that allows a proof of injectivity.
+   *)
   Theorem expand_partition_same_size (A: Set) (l: list A) (f: A -> list A) (f_inv: A -> A)
           (seq_A: list A):
     Listing seq_A ->
+    (exists a, In a l) ->
     fn_partition A l f ->
-    (forall e, In (f_inv e) (f e)) ->
-    length (expand_partition A l f) = length seq_A.
+    fn_partition_inverse A l f f_inv ->
+    (forall d, In (f_inv d) l) ->
+    length (expand_partition A l f f_inv) = length seq_A.
   Proof.
-    intros Listing.
-    intros [l_NoDup IsNonEmpty NoOverlap SameLength NoRepeat EveryElementInPartition].
+    intros Listing l_NonEmpty.
+    intros [l_NoDup NoOverlap SameLength NoRepeat EveryElementInPartition].
+    intros PartitionInverse.
     intros InverseWitness.
-    apply (NoDup_injection_length _ _ _ _ snd (fun x => pair (f_inv x) x)).
-    2: apply Listing.
-    (* snd being injective is not straightforward.
-       we need a way to say something more about the structure of the partitions... *)
-    3: {
-      unfold Injective.
-      intros x y.
-      intros eq.
-      inversion eq.
-      reflexivity.
-    }
-    5: auto.
-
-    3: {
-      intros c.
-      unfold expand_partition.
-      rewrite flat_map_concat_map.
-      Search (In _ (concat _)).
-      split; [intros; apply Listing | ];auto.
-      intros H.
-      apply in_concat_append.
-      (* this is awful too *)
-  Abort.
+    apply (NoDup_injection_length _ _ _ _ (fpair_snd _ _) (fun x => fpair_intro f_inv x)).
+    - apply expand_partition_NoDup; try apply fn_partition_intro; auto.
+    - apply Listing.
+    - simple destruct x; simple destruct y; simpl.
+      intros h H; rewrite H; reflexivity.
+    - intros x y H; inversion H; reflexivity.
+    - apply expand_partition_listing; auto.
+      apply fn_partition_intro; auto.
+    - intros d; rewrite expand_partition_in; auto.
+      simpl.
+      split.
+      intros; exists d; tauto.
+      intros; apply Listing.
+      apply fn_partition_intro; auto.
+    - simpl; tauto.
+  Qed.
 
   (* so let's say we have this, can we prove the size? *)
 
